Some work on connecting veric to concurrency

concurrency/common/ClightSemanticsForMachines.v
@@ -31,12 +31,9 @@ Import Cop.
 Arguments sizeof {env} !t / .
 
 (*Semantics*)
-Require Import VST.veric.Clight_new.
-Require Import VST.veric.Clightnew_coop.
 Require Import VST.veric.Clight_core.
 Require Import VST.veric.Clightcore_coop. 
 Require Import VST.sepcomp.event_semantics.
-Require Import VST.veric.Clight_sim.
 
 Set Bullet Behavior "Strict Subproofs".
 
@@ -389,254 +386,289 @@ Proof.
     constructor; eassumption. }
 Qed. 
 
-Section CLN_SEM.
+Section CLC_SEM.
   Definition F: Type := fundef.
   Definition V: Type := type.
   Definition G := genv.
-  Definition C := corestate.
+  Definition C := CC_core.
   Definition getEnv (g:G): Genv.t F V := genv_genv g.
   (* We might want to define this properly or
      factor the machines so we don't need events here. *)
-  
 (** Transition relation *)
-Inductive cl_evstep (ge: Clight.genv): forall (q: corestate) (m: mem) (T:list mem_event) (q': corestate) (m': mem), Prop :=
+Inductive cl_evstep (ge: Clight.genv): forall (q: CC_core) (m: mem) (T:list mem_event) (q': CC_core) (m': mem), Prop :=
 
-  | evstep_assign: forall ve te k m a1 a2 loc ofs v2 v m' T1 T2 T3,
-     type_is_volatile (typeof a1) = false ->
-      eval_lvalueT ge ve te m a1 loc ofs T1 ->
-      eval_exprT ge ve te m a2 v2 T2 ->
-      Cop.sem_cast v2 (typeof a2) (typeof a1) m = Some v ->
+  | evstep_assign:   forall f a1 a2 k e le m loc ofs v2 v m' T1 T2 T3,
+(*     type_is_volatile (typeof a1) = false ->*)
+      eval_lvalueT ge e le m a1 loc ofs T1 ->
+      eval_exprT ge e le m a2 v2 T2 ->
+      sem_cast v2 (typeof a2) (typeof a1) m = Some v ->
       assign_locT ge (typeof a1) m loc ofs v m' T3 ->
-      cl_evstep ge (State ve te (Kseq (Sassign a1 a2):: k)) m (T1++T2++T3) (State ve te k) m'
+      cl_evstep ge (State f (Sassign a1 a2) k e le) m (T1++T2++T3) 
+                  (State f Sskip k e le) m'
 
-  | evstep_set:   forall ve te k m id a v T,
-      eval_exprT ge ve te m a v T ->
-      cl_evstep ge (State ve te (Kseq (Sset id a) :: k)) m T (State ve (PTree.set id v te) k) m
+  | evstep_set:   forall f id a k e le m v T,
+      eval_exprT ge e le m a v T ->
+      cl_evstep ge (State f (Sset id a) k e le) m T
+              (State f Sskip k e (PTree.set id v le)) m
 
-  | evstep_call_internal:   forall ve te k m optid a al tyargs tyres cc vf vargs f m1 ve' le' T1 T2 T3,
-      Cop.classify_fun (typeof a) = Cop.fun_case_f tyargs tyres cc ->
-      eval_exprT ge ve te m a vf T1 ->
-      eval_exprTlist ge ve te m al tyargs vargs T2 ->
-      Genv.find_funct ge vf = Some (Internal f) ->
-      type_of_function f = Tfunction tyargs tyres cc ->
-      list_norepet (var_names f.(fn_params) ++ var_names f.(fn_temps)) ->
+  | evstep_call:   forall f optid a al k e le m tyargs tyres cconv vf vargs fd T1 T2,
+      classify_fun (typeof a) = fun_case_f tyargs tyres cconv ->
+      eval_exprT ge e le m a vf T1 ->
+      eval_exprTlist ge e le m al tyargs vargs T2 ->
+      Genv.find_funct ge vf = Some fd ->
+      type_of_fundef fd = Tfunction tyargs tyres cconv ->
+      cl_evstep ge (State f (Scall optid a al) k e le) m (T1++T2)
+                  (Callstate fd vargs (Kcall optid f e le k)) m
+
+  | evstep_seq:  forall f s1 s2 k e le m,
+      cl_evstep ge (State f (Ssequence s1 s2) k e le) m nil
+                 (State f s1 (Kseq s2 k) e le) m
+
+  | evstep_skip_seq: forall f s k e le m,
+      cl_evstep ge (State f Sskip (Kseq s k) e le) m nil
+              (State f s k e le) m
+
+  | evstep_continue_seq: forall f s k e le m,
+      cl_evstep ge (State f Scontinue (Kseq s k) e le) m nil
+             (State f Scontinue k e le) m
+
+  | evstep_break_seq: forall f s k e le m,
+      cl_evstep ge (State f Sbreak (Kseq s k) e le) m nil
+            (State f Sbreak k e le) m
+
+  | evstep_ifthenelse:  forall f a s1 s2 k e le m v1 b T,
+      eval_exprT ge e le m a v1 T ->
+      bool_val v1 (typeof a) m = Some b ->
+      cl_evstep ge (State f (Sifthenelse a s1 s2) k e le) m T
+            (State f (if b then s1 else s2) k e le) m
+
+  | evstep_loop: forall f s1 s2 k e le m,
+      cl_evstep ge (State f (Sloop s1 s2) k e le) m nil
+            (State f s1 (Kloop1 s1 s2 k) e le) m
+
+  | evstep_skip_or_continue_loop1:  forall f s1 s2 k e le m x,
+      x = Sskip \/ x = Scontinue ->
+      cl_evstep ge (State f x (Kloop1 s1 s2 k) e le) m nil
+            (State f s2 (Kloop2 s1 s2 k) e le) m
+
+  | evstep_break_loop1:  forall f s1 s2 k e le m,
+      cl_evstep ge (State f Sbreak (Kloop1 s1 s2 k) e le) m nil
+             (State f Sskip k e le) m
+
+  | evstep_skip_loop2: forall f s1 s2 k e le m,
+      cl_evstep ge (State f Sskip (Kloop2 s1 s2 k) e le) m nil
+             (State f (Sloop s1 s2) k e le) m
+
+  | evstep_break_loop2: forall f s1 s2 k e le m,
+      cl_evstep ge (State f Sbreak (Kloop2 s1 s2 k) e le) m nil
+            (State f Sskip k e le) m
+
+  | evstep_return_0: forall f k e le m m',
+      Mem.free_list m (blocks_of_env ge e) = Some m' ->
+      cl_evstep ge (State f (Sreturn None) k e le) m
+            (Free (Clight.blocks_of_env ge e)::nil)
+            (Returnstate Vundef (call_cont k)) m'
+
+  | evstep_return_1: forall f a k e le m v v' m' T,
+      eval_exprT ge e le m a v T ->
+      sem_cast v (typeof a) f.(fn_return) m = Some v' ->
+      Mem.free_list m (blocks_of_env ge e) = Some m' ->
+      cl_evstep ge (State f (Sreturn (Some a)) k e le) m
+            (T ++ Free (Clight.blocks_of_env ge e)::nil)
+           (Returnstate v' (call_cont k)) m'
+
+  | evstep_skip_call: forall f k e le m m',
+      is_call_cont k ->
+      Mem.free_list m (blocks_of_env ge e) = Some m' ->
+      cl_evstep ge (State f Sskip k e le) m
+              (Free (Clight.blocks_of_env ge e)::nil)
+              (Returnstate Vundef k) m'
+
+  | evstep_switch: forall f a sl k e le m v n T,
+      eval_exprT ge e le m a v T ->
+      sem_switch_arg v (typeof a) = Some n ->
+      cl_evstep ge (State f (Sswitch a sl) k e le) m T
+            (State f (seq_of_labeled_statement (select_switch n sl)) (Kswitch k) e le) m
+
+  | evstep_skip_break_switch: forall f x k e le m,
+      x = Sskip \/ x = Sbreak ->
+      cl_evstep ge (State f x (Kswitch k) e le) m nil
+             (State f Sskip k e le) m
+  | evstep_continue_switch: forall f k e le m,
+      cl_evstep ge (State f Scontinue (Kswitch k) e le) m nil
+             (State f Scontinue k e le) m
+
+  | evstep_label: forall f lbl s k e le m,
+      cl_evstep ge (State f (Slabel lbl s) k e le) m nil
+             (State f s k e le) m
+
+  | evstep_goto: forall f lbl k e le m s' k',
+      find_label lbl f.(fn_body) (call_cont k) = Some (s', k') ->
+      cl_evstep ge (State f (Sgoto lbl) k e le) m nil
+             (State f s' k' e le) m
+
+  | evstep_internal_function: forall f vargs k m e le m1 T,
+       list_norepet (var_names (fn_params f)) ->
+       list_disjoint (var_names (fn_params f)) (var_names (fn_temps f)) ->
       forall (NRV: list_norepet (var_names f.(fn_vars))),
-      alloc_variablesT ge empty_env m (f.(fn_vars)) ve' m1 T3 ->
+      alloc_variablesT ge empty_env m (f.(fn_vars)) e m1 T ->
       bind_parameter_temps f.(fn_params) vargs (create_undef_temps f.(fn_temps)) = Some
-le' ->
-      cl_evstep ge (State ve te (Kseq (Scall optid a al) :: k)) m (T1++T2++T3)
-                   (State ve' le' (Kseq f.(fn_body) :: Kseq (Sreturn None) :: Kcall optid f ve te :: k)) m1
+le ->
+      cl_evstep ge (Callstate (Internal f) vargs k) m T
+            (State f f.(fn_body) k e le) m1
 
-  | evstep_call_external:   forall ve te k m optid a al tyargs tyres cc vf vargs ef T1 T2,
-      Cop.classify_fun (typeof a) = Cop.fun_case_f tyargs tyres cc ->
-      eval_exprT ge ve te m a vf T1 ->
-      eval_exprTlist ge ve te m al tyargs vargs T2 ->
-      Genv.find_funct ge vf = Some (External ef tyargs tyres cc) ->
-      cl_evstep ge (State ve te (Kseq (Scall optid a al) :: k)) m (T1++T2) (ExtCall ef vargs optid ve te k) m
+  | evstep_external_function: forall ef targs tres cconv vargs k m t vres m' T
+          (EFI: ef_inline ef = true)
+          (EC: Events.external_call ef ge vargs m t vres m'),
+      T = proj1_sig (inline_external_call_mem_events _ _ _ _ _ _ _ EFI EC) ->
+      cl_evstep ge (Callstate (External ef targs tres cconv) vargs k) m T
+          (Returnstate vres k) m'
 
-  | evstep_seq: forall ve te k m s1 s2 st' m' T,
-          cl_evstep ge (State ve te (Kseq s1 :: Kseq s2 :: k)) m T st' m' ->
-          cl_evstep ge (State ve te (Kseq (Ssequence s1 s2) :: k)) m T st' m'
+  | evstep_returnstate: forall v optid f e le k m,
+      cl_evstep ge (Returnstate v (Kcall optid f e le k)) m nil
+           (State f Sskip k e (set_opttemp optid v le)) m.
 
-  | evstep_skip: forall ve te k m st' m' T,
-          cl_evstep ge (State ve te k) m T st' m' ->
-          cl_evstep ge (State ve te (Kseq Sskip :: k)) m T st' m'
-
-  | evstep_continue: forall ve te k m st' m' T,
-           cl_evstep ge (State ve te (continue_cont k)) m T st' m' ->
-           cl_evstep ge (State ve te (Kseq Scontinue :: k)) m T st' m'
-
-  | evstep_break: forall ve te k m st' m' T,
-                   cl_evstep ge (State ve te (break_cont k)) m T st' m' ->
-                   cl_evstep ge (State ve te (Kseq Sbreak :: k)) m T st' m'
-
-  | evstep_ifthenelse:  forall ve te k m a s1 s2 v1 b T,
-      eval_exprT ge ve te m a v1 T ->
-      Cop.bool_val v1 (typeof a) m = Some b ->
-      cl_evstep ge (State ve te (Kseq (Sifthenelse a s1 s2) :: k)) m T (State ve te  (Kseq (if b then s1 else s2) :: k)) m
-
-  | evstep_for: forall ve te k m s1 s2,
-      cl_evstep ge (State ve te (Kseq (Sloop s1 s2) :: k)) m nil
-              (State ve te (Kseq s1 :: Kseq Scontinue :: Kloop1 s1 s2 :: k)) m
-
-  | evstep_loop2: forall ve te k m a3 s,
-      cl_evstep ge (State ve te (Kloop2 s a3 :: k)) m nil
-             (State ve te (Kseq s :: Kseq Scontinue :: Kloop1 s a3 :: k)) m
-
-  | evstep_return: forall f ve te optexp optid k m v' m' ve' te' te'' k' T,
-      call_cont k = Kcall optid f ve' te' :: k' ->
-      Mem.free_list m (Clight.blocks_of_env ge ve) = Some m' ->
-      match optexp with None => v' = Vundef /\ T=nil
-                      | Some a => exists v, eval_exprT ge ve te m a v T
-                                     /\ Cop.sem_cast v (typeof a) f.(fn_return) m = Some v'
-                            end ->
-      match optid with None => True /\ te''=te'
-                     | Some id => True /\ te'' = PTree.set id v' te'
-      end ->
-      cl_evstep ge (State ve te (Kseq (Sreturn optexp) :: k)) m
-                   (T ++ (Free (Clight.blocks_of_env ge ve)::nil))
-                   (State ve' te'' k') m'
-
-  | evstep_switch: forall ve te k m a sl v n T,
-      eval_exprT ge ve te m a v T ->
-      Cop.sem_switch_arg v (typeof a) = Some n ->
-      cl_evstep ge (State ve te (Kseq (Sswitch a sl) :: k)) m T
-              (State ve te (Kseq (seq_of_labeled_statement (select_switch n sl)) :: Kswitch :: k)) m
-
-  | evstep_label: forall ve te k m lbl s st' m' T,
-       cl_evstep ge (State ve te (Kseq s :: k)) m T st' m' ->
-       cl_evstep ge (State ve te (Kseq (Slabel lbl s) :: k)) m T st' m'
-
-  | evstep_goto: forall f ve te k m lbl k'
-                     (* make sure to take a step here, so that every loop ticks the clock *)
-      (CUR: current_function k = Some f),
-      find_label lbl f.(fn_body) (Kseq (Sreturn None) :: (call_cont k)) = Some k' ->
-      cl_evstep ge (State ve te (Kseq (Sgoto lbl) :: k)) m nil (State ve te k') m.
-
-  Lemma CLN_evstep_ax1 ge : forall c m T c' m' (H: cl_evstep ge c m T c' m' ),
-    corestep (CLN_memsem ge) c m c' m'.
+  Lemma CLC_evstep_ax1 ge : forall c m T c' m' (H: cl_evstep ge c m T c' m' ),
+    corestep (CLC_memsem ge) c m c' m'.
   Proof.
     induction 1; try solve [econstructor; eassumption].
-    { apply eval_lvalueT_ax1 in H0. apply eval_exprT_ax1 in H1.
-      apply assign_locT_ax1 in H3. econstructor; eauto. }
-    { apply eval_exprT_ax1 in H. econstructor; eauto. }
-    { apply eval_exprT_ax1 in H0.
-      apply eval_exprTlist_ax1 in H1.
-      apply alloc_variablesT_ax1 in H5. econstructor; eauto. }
-    { apply eval_exprT_ax1 in H0.
-      apply eval_exprTlist_ax1 in H1. econstructor; eauto. }
-    { apply eval_exprT_ax1 in H. econstructor; eauto. }
-    { destruct optexp.
-      + destruct H1 as [v [E C]]. apply eval_exprT_ax1 in E.
-        econstructor; eauto.
-      + destruct H1; subst. econstructor; eauto. }
-    { apply eval_exprT_ax1 in H. econstructor; eauto. }
+    +  apply eval_lvalueT_ax1 in H. apply eval_exprT_ax1 in H0.
+         apply assign_locT_ax1 in H2. econstructor; eauto.
+    +  apply eval_exprT_ax1 in H. econstructor; eauto.
+    + apply eval_exprT_ax1 in H0.
+      apply eval_exprTlist_ax1 in H1. econstructor; eauto.
+    +  apply eval_exprT_ax1 in H. econstructor; eauto.
+    +  apply eval_exprT_ax1 in H. econstructor; eauto.
+    +  apply eval_exprT_ax1 in H. econstructor; eauto.
+    +  apply alloc_variablesT_ax1 in H1. econstructor; eauto.
+         econstructor; eauto.
   Qed.   
   
-  Lemma CLN_evstep_ax2 ge : forall c m c' m' (H:corestep (CLN_memsem ge) c m c' m'),
+  Lemma CLC_evstep_ax2 ge : forall c m c' m' (H:corestep (CLC_memsem ge) c m c' m'),
       exists T : list mem_event, cl_evstep ge c m T c' m'.
   Proof.
-    induction 1; try solve [ destruct IHcl_step as [T HT]; eexists; econstructor; eauto]; try solve [eexists; econstructor; eauto]. 
-    { apply eval_lvalueT_ax2 in H0. destruct H0 as [T1 A1].
-      apply eval_exprT_ax2 in H1. destruct H1 as [T2 A2].
-      apply assign_locT_ax2 in H3. destruct H3 as [T3 A3].
-      eexists; econstructor; eauto. }
-    { apply eval_exprT_ax2 in H. destruct H as [T H].
-      eexists; econstructor; eauto. }
-    { apply eval_exprT_ax2 in H0. destruct H0 as [T1 K1].
+    induction 1; try solve [ destruct IHcl_step as [T HT]; eexists; econstructor; eauto];
+      try solve [eexists; econstructor; eauto]. 
+  + apply eval_lvalueT_ax2 in H. destruct H as [T1 A1].
+      apply eval_exprT_ax2 in H0. destruct H0 as [T2 A2].
+      apply assign_locT_ax2 in H2. destruct H2 as [T3 A3].
+      eexists; econstructor; eauto.
+  + apply eval_exprT_ax2 in H; destruct H as [T H].
+      eexists; econstructor; eauto.
+  + apply eval_exprT_ax2 in H0. destruct H0 as [T1 K1].
       apply eval_exprTlist_ax2 in H1. destruct H1 as [T2 K2].
-      apply alloc_variablesT_ax2 in H5. destruct H5 as [T3 K3].
-      eexists; econstructor; eauto. }
-    { apply eval_exprT_ax2 in H0. destruct H0 as [T1 K1].
-      apply eval_exprTlist_ax2 in H1. destruct H1 as [T2 K2].
-      eexists; econstructor; eauto. }
-    { apply eval_exprT_ax2 in H. destruct H as [T KT].
-      eexists; econstructor; eauto. }
-    { destruct optexp.
-      + destruct H1 as [v [E C]].
-        apply eval_exprT_ax2 in E. destruct E as [T HT].
-        eexists. econstructor; eauto.
-      + subst. eexists. econstructor; eauto. }
-    { apply eval_exprT_ax2 in H. destruct H as [T K].
-      eexists; econstructor; eauto. }
+      eexists; econstructor; eauto.
+  + apply eval_exprT_ax2 in H; destruct H as [T H].
+      eexists; econstructor; eauto.
+  + apply eval_exprT_ax2 in H; destruct H as [T H].
+      eexists; econstructor; eauto.
+  + apply eval_exprT_ax2 in H; destruct H as [T H].
+      eexists; econstructor; eauto.
+  + inv H. apply alloc_variablesT_ax2 in H3. destruct H3 as [T3 K3].
+      eexists; econstructor; eauto.
+Unshelve.
+3: eassumption.
+auto.
 Qed.
 
-  Lemma CLN_evstep_fun ge : forall c m T' c' m' T'' c'' m''
+  Lemma CLC_evstep_fun ge : forall c m T' c' m' T'' c'' m''
                                    (K: cl_evstep ge c m T' c' m') (K': cl_evstep ge c m T'' c'' m''), T' = T''.
   Proof. intros. generalize dependent m''. generalize dependent c''. generalize dependent T''.
          induction K; simpl; intros; try solve [ inv K'; eauto ].
-  { inv K'. exploit eval_exprT_fun. apply H15. apply H1. intros X; inv X.
-    exploit eval_lvalueT_fun. apply H14. apply H0. intros X; inv X.
-    rewrite H16 in H2; inv H2.
-    exploit assign_locT_fun. apply H17. apply H3. intros X; inv X; trivial. }
-  { inv K'. exploit eval_exprT_fun. apply H9. apply H. intros X; inv X. trivial. }
-  { inv K'.
-    + rewrite H13 in H; inv H.
-      exploit eval_exprT_fun. apply H14. apply H0. intros X; inv X.
-      exploit eval_exprTlist_fun. apply H15. apply H1. intros X; inv X.
-      rewrite H20 in H2; inv H2.
-      rewrite H24 in H6; inv H6.
-      exploit alloc_variablesT_fun. apply H23. apply H5.
-      intros X; inv X; trivial.
-    + rewrite H17 in H; inv H.
-      exploit eval_exprT_fun. apply H18. apply H0. intros X; inv X.
-      congruence. }
-  { inv K'.
-    + rewrite H9 in H; inv H.
-      exploit eval_exprT_fun. apply H10. apply H0. intros X; inv X.
-      congruence.
-    + rewrite H13 in H; inv H.
-      exploit eval_exprT_fun. apply H14. apply H0. intros X; inv X.
-      exploit eval_exprTlist_fun. apply H15. apply H1. intros X; inv X.
-      congruence. }
-  { inv K'.
-    exploit eval_exprT_fun. apply H11. apply H. intros X; inv X. trivial. }
-  { inv K'. destruct optexp.
-    + destruct H1 as [u [E C]]. destruct H13 as [u' [E' C']].
-      exploit eval_exprT_fun. apply E'. apply E. intros X; inv X. trivial.
-    + destruct H1; destruct H13; subst. trivial. }
-  { inv K'.
-    exploit eval_exprT_fun. apply H10. apply H. intros X; inv X. trivial. }
-  Qed.
+ - inv K'. exploit eval_exprT_fun. apply H14. apply H0. intros X; inv X.
+    exploit eval_lvalueT_fun. apply H13. apply H. intros X; inv X.
+    rewrite H15 in H1; inv H1.
+    exploit assign_locT_fun. apply H16. apply H2. intros X; inv X; trivial.
+   destruct H12; discriminate.
+   destruct H12; discriminate.
+ - inv K'. exploit eval_exprT_fun. apply H10. apply H. intros X; inv X. trivial.
+    destruct H9; discriminate.
+    destruct H9; discriminate.
+ - inv K'.
+    + rewrite H15 in H; inv H.
+      exploit eval_exprT_fun. eassumption. apply H0. intros X; inv X.
+      exploit eval_exprTlist_fun. eassumption. apply H1. intros X; inv X.
+      rewrite H18 in H2; inv H2.
+      rewrite H19 in H3; inv H3. auto.
+    + destruct H13; discriminate.
+    + destruct H13; discriminate.
+ - inv K'; auto. contradiction.
+ - inv K'. exploit eval_exprT_fun. eassumption. eapply H. intros X; inv X. auto.
+    destruct H10; discriminate.
+    destruct H10; discriminate.
+ - destruct H; subst x; inv K'; auto. contradiction.
+ - inv K'; auto; contradiction.
+ - inv K'; try solve [destruct H9; discriminate]. inversion2 H H8. auto.
+ - inv K'; try solve [destruct H11; discriminate].
+    exploit eval_exprT_fun. eassumption. eapply H. intros X; inv X. auto.
+ - inv K'; try contradiction. auto.
+ - inv K'; try solve [destruct H10; discriminate].
+    exploit eval_exprT_fun. eassumption. eapply H. intros X; inv X. auto.
+ - destruct H; subst x; inv K'; auto. contradiction.
+ - inv K'. 
+      exploit alloc_variablesT_fun. eassumption. apply H1. intros X; inv X. auto.
+ - inv K'. simpl.
+Abort.
 
-  Lemma CLN_evstep_elim ge : forall c m T c' m' (K: cl_evstep ge c m T c' m'),
+  Lemma CLC_evstep_elim ge : forall c m T c' m' (K: cl_evstep ge c m T c' m'),
         ev_elim m T m'.
   Proof.
     induction 1; try solve [constructor];
       try solve [ apply eval_exprT_elim in H; trivial]; trivial.
-    { eapply assign_locT_elim in H3. destruct H3 as [EV3 _ ].
-      eapply eval_lvalueT_elim in H0.
-      eapply eval_exprT_elim in H1.
-      eapply ev_elim_app; eauto. eapply ev_elim_app; eauto. }
-    { apply eval_exprT_elim in H0.
+  + eapply assign_locT_elim in H2. destruct H2 as [EV3 _ ].
+      eapply eval_lvalueT_elim in H.
+      eapply eval_exprT_elim in H0.
+      eapply ev_elim_app; eauto. eapply ev_elim_app; eauto.
+  + apply eval_exprT_elim in H0.
       apply eval_exprTlist_elim in H1.
-      apply alloc_variablesT_elim in H5; destruct H5 as [? _].
-      eapply ev_elim_app; eauto. eapply ev_elim_app; eauto. }
-    { apply eval_exprT_elim in H0.
-      apply eval_exprTlist_elim in H1.
-      eapply ev_elim_app; eauto. }
-    { destruct optexp.
-      + destruct H1 as [? [? ?]]. apply eval_exprT_elim in H1.
-        eapply ev_elim_app; [ eassumption | simpl].
-        exists m'; split; trivial.
-      + destruct H1; subst; simpl. exists m'; split; trivial. }
+      eapply ev_elim_app; eauto.
+  + eexists; split; eauto. reflexivity.
+  + apply eval_exprT_elim in H.
+      eapply ev_elim_app; eauto.
+      eexists; split; eauto. reflexivity.
+  + eexists; split; eauto. reflexivity.
+  + apply alloc_variablesT_elim in H1.
+      destruct H1; auto.
+  + destruct  (inline_external_call_mem_events ef ge vargs m t
+         vres m' EFI EC). simpl in H. subst x. auto.
   Qed.
   
   (** *Event semantics for Clight_new*)
    (* This should be a version of CLN_memsem annotated with memory events.*)
   
-  Program Definition CLN_evsem ge : @EvSem C := {| msem := CLN_memsem ge; ev_step := cl_evstep ge |}.
-  Next Obligation. apply CLN_evstep_ax1. Qed.
-  Next Obligation. apply CLN_evstep_ax2. Qed.
-  Next Obligation. apply CLN_evstep_fun. Qed.
-  Next Obligation. apply CLN_evstep_elim. Qed.  
+  Program Definition CLC_evsem ge : @EvSem C := {| msem := CLC_memsem ge; ev_step := cl_evstep ge |}.
+  Next Obligation. apply CLC_evstep_ax1. Qed.
+  Next Obligation. apply CLC_evstep_ax2. Qed.
+(*  Next Obligation. apply CLC_evstep_fun. Qed. *)
+  Next Obligation. apply CLC_evstep_elim. Qed.  
 
-  Lemma CLN_msem : forall ge, msem (CLN_evsem ge) = CLN_memsem ge.
+  Lemma CLC_msem : forall ge, msem (CLC_evsem ge) = CLC_memsem ge.
   Proof. auto. Qed.
-End CLN_SEM.
+End CLC_SEM.
 
-  Lemma CLN_step_decay: forall g c m tr c' m',
-      event_semantics.ev_step (CLN_evsem g) c m tr c' m' ->
+  Lemma CLC_step_decay: forall g c m tr c' m',
+      event_semantics.ev_step (CLC_evsem g) c m tr c' m' ->
       decay m m'.
 Proof.
 intros.
-pose proof (msem_decay (CLN_memsem g) c m c' m').
+pose proof (msem_decay (CLC_memsem g) c m c' m').
 apply H0. clear H0.
 simpl in *.
-apply CLN_evstep_ax1 in H.
+apply CLC_evstep_ax1 in H.
 auto.
 Qed.
 
   Lemma at_external_SEM_eq:
-     forall ge c m, semantics.at_external (CLN_evsem ge) c m =
-      match c with
-      | State _ _ _ => None
-      | ExtCall ef args _ _ _ _ => Some (ef, args)
-      end.
+     forall ge c m, semantics.at_external (CLC_evsem ge) c m =
+     match c with
+     | Callstate (External ef _ _ _) args _ => 
+         if ef_inline ef then None else Some (ef, args)
+     | _ => None
+   end.
   Proof. auto. Qed.
 
-  Instance Clight_newSem ge : Semantics :=
-    { semG := G; semC := C; semSem := CLN_evsem ge; the_ge := ge }.
+  Instance ClightSem ge : Semantics :=
+    { semG := G; semC := C; semSem := CLC_evsem ge; the_ge := ge }.
 
   Inductive builtin_event: external_function -> mem -> list val -> list mem_event -> Prop :=
   BE_malloc: forall m n m'' b m'
@@ -704,346 +736,6 @@ inversion BE1; inv BE2; try discriminate; try contradiction; simpl in *; trivial
 + inv H3; inv H5.
   rewrite LB0 in LB; inv LB; trivial.
 Qed.
-
-Section CLC_SEM.
-  Variable g: Clight.genv.
-    
-  Section CLC_step.
-    Variable function_entryT: function -> list val -> mem -> env -> temp_env -> mem -> list mem_event -> Prop.
-
-    Inductive clc_evstep: state -> mem -> list mem_event -> state -> mem -> Prop :=
-  | clc_evstep_assign: forall f a1 a2 k e le m loc ofs v2 v m' T1 T2 T3 mx,
-      eval_lvalueT g e le m a1 loc ofs T1 ->
-      eval_exprT g e le m a2 v2 T2 ->
-      sem_cast v2 (typeof a2) (typeof a1) m = Some v ->
-      assign_locT g (typeof a1) m loc ofs v m' T3 ->
-      clc_evstep (Clight.State f (Sassign a1 a2) k e le mx) m (T1++T2++T3)
-                 (Clight.State f Sskip k e le m') m'
-
-  | clc_evstep_set: forall f id a k e le m v T mx,
-      eval_exprT g e le m a v T ->
-      clc_evstep (Clight.State f (Sset id a) k e le mx) m
-        T (Clight.State f Sskip k e (PTree.set id v le) m) m
-
-  | clc_evstep_call: forall f optid a al k e le m tyargs tyres cconv vf vargs fd T1 T2 mx,
-      classify_fun (typeof a) = fun_case_f tyargs tyres cconv ->
-      eval_exprT g e le m a vf T1 ->
-      eval_exprTlist g e le m al tyargs vargs T2 ->
-      Genv.find_funct g vf = Some fd ->
-      type_of_fundef fd = Tfunction tyargs tyres cconv ->
-      clc_evstep (Clight.State f (Scall optid a al) k e le mx) m 
-        (T1++T2) (Clight.Callstate fd vargs (Clight.Kcall optid f e le k) m) m
-
-  | clc_evstep_builtin: forall f optid ef tyargs al k e le m vargs t vres m' T1 T2 mx,
-      eval_exprTlist g e le m al tyargs vargs T1 ->
-      builtin_event ef m vargs T2 ->
-      Events.external_call ef g vargs m t vres m' ->
-      clc_evstep (Clight.State f (Sbuiltin optid ef tyargs al) k e le mx) m
-                 (T1++T2) (Clight.State f Sskip k e (set_opttemp optid vres le) m') m'
-    
-  | clc_evstep_seq:  forall f s1 s2 k e le m mx,
-      clc_evstep (Clight.State f (Ssequence s1 s2) k e le mx) m
-        nil (Clight.State f s1 (Clight.Kseq s2 k) e le m) m
-  | clc_evstep_skip_seq: forall f s k e le m mx,
-      (*~ is_call_cont k ->*)
-      clc_evstep (Clight.State f Sskip (Clight.Kseq s k) e le mx) m
-        nil (Clight.State f s k e le m) m
-  | clc_evstep_continue_seq: forall f s k e le m mx,
-      clc_evstep (Clight.State f Scontinue (Clight.Kseq s k) e le mx) m
-        nil (Clight.State f Scontinue k e le m) m
-  | clc_evstep_break_seq: forall f s k e le m mx,
-      clc_evstep (Clight.State f Sbreak (Clight.Kseq s k) e le mx) m
-        nil (Clight.State f Sbreak k e le m) m
-
-  | clc_evstep_ifthenelse:  forall f a s1 s2 k e le m v1 b T mx,
-      eval_exprT g e le m a v1 T ->
-      bool_val v1 (typeof a) m = Some b ->
-      clc_evstep (Clight.State f (Sifthenelse a s1 s2) k e le mx) m
-        T (Clight.State f (if b then s1 else s2) k e le m) m
-
-  | clc_evstep_loop: forall f s1 s2 k e le m mx,
-      clc_evstep (Clight.State f (Sloop s1 s2) k e le mx) m
-        nil (Clight.State f s1 (Clight.Kloop1 s1 s2 k) e le m) m
-  | clc_evstep_skip_or_continue_loop1:  forall f s1 s2 k e le m x mx,
-      x = Sskip \/ x = Scontinue ->
-      clc_evstep (Clight.State f x (Clight.Kloop1 s1 s2 k) e le mx) m
-        nil (Clight.State f s2 (Clight.Kloop2 s1 s2 k) e le m) m
-  | clc_evstep_break_loop1:  forall f s1 s2 k e le m mx,
-      clc_evstep (Clight.State f Sbreak (Clight.Kloop1 s1 s2 k) e le mx) m
-        nil (Clight.State f Sskip k e le m) m
-  | clc_evstep_skip_loop2: forall f s1 s2 k e le m mx,
-      clc_evstep (Clight.State f Sskip (Clight.Kloop2 s1 s2 k) e le mx) m
-        nil (Clight.State f (Sloop s1 s2) k e le m) m
-  | clc_evstep_break_loop2: forall f s1 s2 k e le m mx,
-      clc_evstep (Clight.State f Sbreak (Clight.Kloop2 s1 s2 k) e le mx) m
-                 nil (Clight.State f Sskip k e le m) m
-                 
-  | clc_evstep_return_0: forall f k e le m m' mx,
-      Mem.free_list m (blocks_of_env g e) = Some m' ->
-      clc_evstep (Clight.State f (Sreturn None) k e le mx) m
-        (Free (blocks_of_env g e)::nil) (Returnstate Vundef (Clight.call_cont k) m') m'
-  | clc_evstep_return_1: forall f a k e le m v v' m' T mx,
-      eval_exprT g e le m a v T ->
-      sem_cast v (typeof a) f.(fn_return) m = Some v' ->
-      Mem.free_list m (blocks_of_env g e) = Some m' ->
-      clc_evstep (Clight.State f (Sreturn (Some a)) k e le mx) m
-        (T++Free (blocks_of_env g e)::nil) (Returnstate v' (Clight.call_cont k) m') m'
-  | clc_evstep_skip_call: forall f k e le m m' mx,
-      is_call_cont k ->
-      Mem.free_list m (blocks_of_env g e) = Some m' ->
-      clc_evstep (Clight.State f Sskip k e le mx) m
-        (Free (blocks_of_env g e)::nil) (Returnstate Vundef k m') m'
-
-  | clc_evstep_switch: forall f a sl k e le m v n T mx,
-      eval_exprT g e le m a v T ->
-      sem_switch_arg v (typeof a) = Some n ->
-      clc_evstep (Clight.State f (Sswitch a sl) k e le mx) m
-        T (Clight.State f (seq_of_labeled_statement (select_switch n sl)) (Clight.Kswitch k) e le m) m
-  | clc_evstep_skip_break_switch: forall f x k e le m mx,
-      x = Sskip \/ x = Sbreak ->
-      clc_evstep (Clight.State f x (Clight.Kswitch k) e le mx) m
-        nil (Clight.State f Sskip k e le m) m
-  | clc_evstep_continue_switch: forall f k e le m mx,
-      clc_evstep (Clight.State f Scontinue (Clight.Kswitch k) e le mx) m
-        nil (Clight.State f Scontinue k e le m) m
-
-  | clc_evstep_label: forall f lbl s k e le m mx,
-      clc_evstep (Clight.State f (Slabel lbl s) k e le mx) m
-        nil (Clight.State f s k e le m) m
-
-  | clc_evstep_goto: forall f lbl k e le m s' k' mx,
-      Clight.find_label lbl f.(fn_body) (Clight.call_cont k) = Some (s', k') ->
-      clc_evstep (Clight.State f (Sgoto lbl) k e le mx) m
-        nil (Clight.State f s' k' e le m) m
-
-  | clc_evstep_internal_function: forall f vargs k m e le m1 T mx,
-      function_entryT f vargs m e le m1 T ->
-      clc_evstep (Clight.Callstate (Internal f) vargs k mx) m
-        T (Clight.State f f.(fn_body) k e le m1) m1
-(*
-  | clc_evstep_external_function: forall ef targs tres cconv vargs k m vres t m',
-      external_call ef ge vargs m t vres m' ->
-      clc_evstep (Clight.Callstate (External ef targs tres cconv) vargs k m)
-         t (Clight.Returnstate vres k m')*)
-
-  | clc_evstep_returnstate: forall v optid f e le k m mx,
-      clc_evstep (Clight.Returnstate v (Clight.Kcall optid f e le k) mx) m
-        nil (Clight.State f Sskip k e (set_opttemp optid v le) m) m.
-
-  Lemma clc_ax1 
-        (HFe: forall f vargs m e le m1 T,
-            function_entryT f vargs m e le m1 T -> function_entry2 g f vargs m e le m1):
-    forall c m T c' m', clc_evstep c m T c' m' ->
-        Clight.at_external (set_mem c m) = None /\
-        m' = get_mem c' /\
-        exists t, step g (function_entry2 g) (set_mem c m) t c'.
-  Proof.
-    induction 1; simpl; split; trivial; split; trivial; intros;
-     try solve [ apply eval_exprT_ax1 in H; eexists; econstructor; eauto ];
-     try solve [ eexists; econstructor; eauto ].
-    { apply eval_lvalueT_ax1 in H. apply eval_exprT_ax1 in H0.
-      apply assign_locT_ax1 in H2. eexists; econstructor; eauto. }
-    { apply eval_exprT_ax1 in H0. apply eval_exprTlist_ax1 in H1.
-      eexists; econstructor; eauto. }
-    { apply eval_exprTlist_ax1 in H. 
-      eexists; econstructor; eauto. }
-  Qed.
-  
-  Lemma clc_ax2
-        (Hfe: forall f vargs m e le m1, function_entry2 g f vargs m e le m1 ->
-            exists T, function_entryT f vargs m e le m1 T):
-        forall d t c' 
-                        (H: step g (function_entry2 g) d t c')
-                        c m (HD : d = set_mem c m)
-                        (AE : Clight.at_external d = None),
-      exists T : list mem_event, clc_evstep c m T c' (get_mem c').
-  Proof.
-    induction 1; simpl; intros; destruct c; inv HD; simpl in *;
-      try solve [eexists; econstructor; eauto]; try solve [congruence].
-    { apply eval_lvalueT_ax2 in H; destruct H as [T1 K1].
-      apply eval_exprT_ax2 in H0; destruct H0 as [T2 A2].
-      apply assign_locT_ax2 in H2; destruct H2 as [T3 A3].
-      eexists. econstructor; eauto. }
-    { apply eval_exprT_ax2 in H. destruct H as [T H].
-      eexists. eapply clc_evstep_set; eauto. }
-    { apply eval_exprT_ax2 in H0. destruct H0 as [T1 K1].
-      apply eval_exprTlist_ax2 in H1. destruct H1 as [T2 K2].
-      eexists; eapply clc_evstep_call; eauto. }
-    { apply eval_exprTlist_ax2 in H. destruct H as [T1 K1].
-      assert (BE: exists T2, builtin_event ef m0 vargs T2).
-      { destruct ef; try solve [ exists nil; econstructor; eauto].
-        { (*EF_malloc*) inv H0. exploit Mem.store_valid_access_3; eauto. intros [_ ALGN].
-          apply Mem.store_storebytes in H1.
-          eexists. eapply BE_malloc; eauto. }
-        { (*EF_free*) inv H0. exploit Mem.load_valid_access; eauto. intros [_ ALGN].
-          exploit Mem.load_loadbytes; eauto. intros [bytes [LD X]].
-          eexists. eapply BE_free; eauto. }
-        { (*EF_memcpy*) inv H0.
-          eexists. eapply BE_memcpy; eauto. } } 
-      destruct BE as [T2 BE].
-      eexists; econstructor; eauto. }
-    { apply eval_exprT_ax2 in H. destruct H as [T HT].
-      eexists; econstructor; eauto. }
-    { apply eval_exprT_ax2 in H. destruct H as [T HT].
-      eexists; econstructor; eauto. }
-    { apply eval_exprT_ax2 in H. destruct H as [T HT].
-      eexists; econstructor; eauto. }
-    { apply Hfe in H; destruct H as [T HT].
-      eexists. econstructor; eauto. }
-  Qed.
-
-  Lemma clc_fun (HFe: forall f vargs m e1 le1 m1 T1 (FE1:function_entryT f vargs m e1 le1 m1 T1)
-                             e2 le2 m2 T2 (FE2:function_entryT f vargs m e2 le2 m2 T2), T1=T2):
-    forall c m T1 c1 m1 T2 c2 m2 (EX1: clc_evstep c m T1 c1 m1)
-           (EX2:clc_evstep c m T2 c2 m2), T1 = T2.
-  Proof.
-    induction 1; simpl; intros; try solve [inv EX2; split; reflexivity].
-    { inv EX2. exploit eval_lvalueT_fun. apply H14. apply H. intros X; inv X.
-      exploit eval_exprT_fun. apply H15. apply H0. intros X; inv X.
-      rewrite H16 in H1; inv H1.
-      exploit assign_locT_fun. apply H17. apply H2. intros X; inv X. trivial.
-      destruct H13; subst; congruence.
-      destruct H13; subst; congruence. }
-    { inv EX2. exploit eval_exprT_fun. apply H11. apply H. intros X; inv X. trivial.
-      destruct H10; subst; congruence.
-      destruct H10; subst; congruence. } 
-    { inv EX2.
-      { rewrite H16 in H; inv H.
-        exploit eval_exprT_fun. apply H17. apply H0. intros X; inv X.
-        exploit eval_exprTlist_fun. apply H18. apply H1. intros X; inv X. trivial. }
-      destruct H14; subst; congruence.
-      destruct H14; subst; congruence. }
-    { inv EX2.
-      { exploit eval_exprTlist_fun. apply H15. apply H. intros X; inv X.
-        exploit builtin_event_determ. apply H16. apply H0. congruence. }
-      destruct H12; congruence. 
-      destruct H12; congruence. }
-    { inv EX2. trivial. contradiction. }
-    { inv EX2. 
-      exploit eval_exprT_fun. apply H13. apply H. congruence.
-      destruct H11; congruence. destruct H11; congruence. }
-    { destruct H; subst; inv EX2; trivial. contradiction. }
-    { inv EX2; trivial. contradiction. }
-    { inv EX2. destruct H10; congruence. congruence. destruct H10; congruence. }
-    { inv EX2. destruct H12; congruence.  
-      exploit eval_exprT_fun. apply H12. apply H. congruence.
-      destruct H12; congruence. }
-    { inv EX2; try solve [ contradiction ]; trivial. }
-    { inv EX2. destruct H11; congruence.
-      exploit eval_exprT_fun. apply H12. apply H. congruence.
-      destruct H11; congruence. }
-    { destruct H; subst; inv EX2; try solve [contradiction]; trivial. }
-    { inv EX2. eauto. }
-  Qed.
-
-  Lemma extcall_ev_elim: forall ef g vargs m t vres m' ev
-    (Hext: Events.external_call ef g vargs m t vres m')
-    (Hev: builtin_event ef m vargs ev)
-    (Hef: match ef with EF_malloc | EF_free | EF_memcpy _ _ => False | _ => True end),
-    ev_elim m ev m'.
-  Proof.
-  Admitted.
-
-  Lemma clc_ev_elim (FE: forall f vargs m e le m1 T (E:function_entryT f vargs m e le m1 T), ev_elim m T m1):
-    forall c m T c' m' (E: clc_evstep c m T c' m'), ev_elim m T m'.
-  Proof.
-    induction 1; try solve [constructor];
-      try solve [ apply eval_exprT_elim in H; trivial]; trivial.
-    - eapply assign_locT_elim in H2. destruct H2 as [EV3 _ ].
-      eapply eval_lvalueT_elim in H.
-      eapply eval_exprT_elim in H0.
-      eapply ev_elim_app; eauto. eapply ev_elim_app; eauto.
-    - apply eval_exprT_elim in H0.
-      apply eval_exprTlist_elim in H1.
-      eapply ev_elim_app; eauto.
-    - apply eval_exprTlist_elim in H. eapply ev_elim_app; eauto. clear H.
-      inv H0.
-      { exploit extcall_malloc_sem_inv. apply H1. clear H1. intros [m1 [bb [sz [X [Ht [Hres [A STORE]]]]]]]; subst.
-        assert (HV: Vptrofs n = Vptrofs sz).
-        { clear -X. remember (Vptrofs n). remember  (Vptrofs sz).  clear Heqv Heqv0. inv X; trivial. }
-        rewrite (Vptrofs_inj _ _ HV) in *. rewrite HV in *. clear X.
-        rewrite A in ALLOC. inv ALLOC. apply Mem.store_storebytes in STORE.
-        rewrite ST in STORE. inv STORE.
-        econstructor; split. eassumption. econstructor; split. eassumption. reflexivity. }
-      {  inv H1. apply Mem.load_loadbytes in H2. destruct H2 as [bytes1 [LD V]]; subst.
-         rewrite LD in LB; inv LB. rewrite <- SZ in V. rewrite (Vptrofs_inj _ _ V) in *. clear V SZ.
-         rewrite FR in H8; inv H8.
-         econstructor. eassumption. econstructor. split. { simpl. rewrite FR. reflexivity. } reflexivity. }
-      { inv H1. rewrite H14 in LB; inv LB. rewrite ST in H15; inv H15.
-        econstructor. eassumption. econstructor; split. eassumption. reflexivity. }
-      eapply extcall_ev_elim; eauto; constructor; auto.
-    - do 2 eexists; eauto; constructor.
-    - apply eval_exprT_elim in H.
-      eapply ev_elim_app; eauto.
-      do 2 eexists; eauto; constructor.
-    - do 2 eexists; eauto; constructor.
-    - eauto.
-  Qed.
-
-End CLC_step.
-
-  Inductive function_entryT2 (f: function) (vargs: list val) (m: mem) (e: env) (le: temp_env) (m': mem) (T:list mem_event): Prop :=
-  | function_entry2_intro:
-      list_norepet (var_names f.(fn_vars)) ->
-      list_norepet (var_names f.(fn_params)) ->
-      list_disjoint (var_names f.(fn_params)) (var_names f.(fn_temps)) ->
-      alloc_variablesT g empty_env m f.(fn_vars) e m' T ->
-      bind_parameter_temps f.(fn_params) vargs (create_undef_temps f.(fn_temps)) = Some le ->
-      function_entryT2 f vargs m e le m' T. 
-
-  Lemma Hfe2_ax1 f vargs m e le m1 T (FE: function_entryT2 f vargs m e le m1 T):
-    function_entry2 g f vargs m e le m1.
-  Proof. inv FE. apply alloc_variablesT_ax1 in H2. econstructor; eauto. Qed.
-
-  Lemma Hfe2_ax2 f vargs m e le m1 (FE: function_entry2 g f vargs m e le m1):
-    exists T, function_entryT2 f vargs m e le m1 T.
-  Proof. inv FE. apply alloc_variablesT_ax2 in H2. destruct H2 as [T HT].
-         eexists; econstructor; eauto.
-  Qed.
-
-  Lemma Hfe2_fun f vargs m e1 le1 m1 T1 (FE1: function_entryT2 f vargs m e1 le1 m1 T1)
-        e2 le2 m2 T2 (FE2: function_entryT2 f vargs m e2 le2 m2 T2): (e1,m1,T1)=(e2,m2,T2).
-  Proof. inv FE1. inv FE2.
-         exploit alloc_variablesT_fun. apply H7. apply H2. congruence.
-  Qed.
-  
-  Lemma Hfe2_ev_elim f vargs m e le m1 T (FE: function_entryT2 f vargs m e le m1 T): ev_elim m T m1.
-  Proof. inv FE. eapply alloc_variablesT_elim. eassumption. Qed. 
-
-  Program Definition CLC_evsem : @EvSem state := {| msem := CLC_memsem g; ev_step := clc_evstep function_entryT2 |}.
-  Next Obligation. simpl. intros. unfold part_semantics2; simpl.
-                   apply clc_ax1 in H. destruct H as [AE [? [t Ht]]]; subst.
-                   econstructor; simpl; trivial. apply Ht. apply Hfe2_ax1. Qed.
-  Next Obligation. simpl. unfold part_semantics2; simpl. intros.
-                   inv H; simpl in *. unfold step2 in H0. simpl in *.
-                   eapply clc_ax2; eauto. apply Hfe2_ax2. Qed.
-  Next Obligation. simpl. unfold part_semantics2; simpl. intros.
-                   eapply clc_fun; try eassumption. intros.
-                   exploit Hfe2_fun. apply FE2. apply FE1. congruence. Qed.
-  Next Obligation. simpl; intros. eapply clc_ev_elim; eauto. apply Hfe2_ev_elim. Qed.
-
-  Lemma CLC_msem : msem CLC_evsem = CLC_memsem g.
-  Proof. auto. Qed.
-
-  Lemma CLC_step_decay: forall c m tr c' m',
-      event_semantics.ev_step (CLC_evsem) c m tr c' m' ->
-      decay m m'.
-Proof.
-intros.
-apply (msem_decay (CLC_memsem g) c m c' m').
-simpl in *.
-apply clc_ax1 in H.
-destruct H as [? [? [t ?]]]; subst.
-exploit (coreify (part_semantics2 g)); eauto.
-intros.
-inv H0.
-constructor; auto.
-eapply alloc_variablesT_ax1; eauto.
-Qed.
-
-  Instance ClightSem : Semantics :=
-    { semG := G; semC := state; semSem := CLC_evsem; the_ge := g }.
-End CLC_SEM.
 
   (* extending Clight_sim to event semantics *)
 Inductive ev_star ge: state -> mem -> _ -> state -> mem -> Prop :=
@@ -1133,667 +825,4 @@ Proof.
   eapply ev_plus_left; eauto. eapply ev_star_trans; eauto.
 Qed.
 
-Lemma exec_skipsT:
- forall ge {s0 k s k'}
-   (H1: match_cont (Kseq s0 :: k) (strip_skip' (CC.Kseq s k')))
-   f ve te m mm,
-   match s0 with Sskip => False | Scontinue => False | Sloop _ _ => False
-            | Sifthenelse _ _ _ => False | Sreturn _ => False
-            | _ => True end ->
-   exists k2 mm', strip_skip' (CC.Kseq s k') = CC.Kseq s0 k2 /\
-     ev_star ge (CC.State f s k' ve te mm) m nil (CC.State f s0 k2 ve te mm') m.
-Proof.
- intros.
- remember (CC.Kseq s k') as k0.
- revert k s k' mm H1 Heqk0; induction k0; intros; inv Heqk0.
- assert ({s1=Sskip}+{s1<>Sskip}) by (destruct s1; try (left; congruence); right; congruence).
- destruct H0.
-{ subst s1.
-  destruct k'; try solve [inv H1].
-  { specialize (IHk0 _ s k' m H1 (eq_refl _)).
-    destruct IHk0 as [k2 [m2 [? ?]]].
-    exists k2, m2. split; simpl; auto.
-    replace nil with ((@nil mem_event)++nil) by reflexivity.
-    econstructor 2. constructor. apply H2. }
-  { inv H1; contradiction. }
-  simpl in *. inv H1. contradiction. }
-{ replace (strip_skip' (CC.Kseq s1 k')) with (CC.Kseq s1 k')  in *
-     by (destruct s1; try congruence; auto).
-  inv H1.
-  exists k', mm; split; auto.
-  constructor 1. }
-Qed.
-
-Lemma strip_evstep:
-  forall ge ve te k m T st' m',
-     cl_evstep ge (State ve te (strip_skip k)) m T st' m' <->
-    cl_evstep ge (State ve te k) m T st' m'.
-Proof.
-intros.
- induction k; intros; split; simpl; intros; try destruct IHk; auto.
- destruct a; try destruct s; auto.
-  constructor; auto.
- destruct a; try destruct s; auto.
- inv H. auto.
-Qed.
-
-Lemma ev_strip_skip'_loop1:
-  forall ge f ve te m a3 s k1 k mm, CC.Kloop1 a3 s k1 = strip_skip' k ->
-  exists mm', ev_star ge (CC.State f Sskip k ve te mm) m nil (CC.State f Sskip (CC.Kloop1 a3 s k1) ve te mm') m.
-Proof.
- induction k; intros; try solve [inv H].
- destruct (dec_skip s0). subst. replace nil with (@nil mem_event++nil) by reflexivity. destruct (IHk m H) as [mm' ?]; exists mm'. eapply ev_star_trans; try eassumption; apply ev_star_one;
-   constructor; eauto.
- rewrite strip_skip'_not in * by auto.
- rewrite <- H. exists mm; constructor 1. simpl in H. inv H. exists mm; constructor 1.
-Qed.
-
-Lemma evstrip_skip'_loop2:
-  forall ge f ve te m a3 s k1 k mm, CC.Kloop2 a3 s k1 = strip_skip' k ->
-  exists mm', ev_star ge (CC.State f Sskip k ve te mm) m nil (CC.State f Sskip (CC.Kloop2 a3 s k1) ve te mm') m.
-Proof.
- induction k; intros; try solve [inv H].
- { destruct (dec_skip s0).
-   { subst. replace nil with (@nil mem_event++nil) by reflexivity.
-     destruct (IHk m H) as [mm' ?]; exists mm'.
-     eapply ev_star_trans; eauto.
-     replace nil with (@nil mem_event++nil) by reflexivity. apply ev_star_one.
-     constructor. }
-   { rewrite strip_skip'_not in * by auto.
-     rewrite <- H. exists mm; constructor 1. } }
- simpl in H. inv H. exists mm; constructor 1.
-Qed.
-
-Lemma evstrip_skip'_call:
-  forall ge f ve te m lid f' ve' te' k1 k mm, CC.Kcall lid f' ve' te' k1 = strip_skip' k ->
-  exists mm', ev_star ge (CC.State f Sskip k ve te mm) m nil (CC.State f Sskip (CC.Kcall lid f' ve' te' k1) ve te mm') m.
-Proof.
- induction k; intros; try solve [inv H].
- destruct (dec_skip s). subst. replace nil with (@nil mem_event++nil) by reflexivity. destruct (IHk m H) as [mm' ?]; exists mm'. eapply ev_star_trans; eauto. apply ev_star_one.
- constructor. auto.
- rewrite strip_skip'_not in * by auto.
- rewrite <- H. exists mm; constructor 1. simpl in H. inv H. exists mm; constructor 1.
-Qed.
-
-Lemma evexec_skips':
-  forall ge f s k' s0 k0' ve te m mm,
-        strip_skip' (CC.Kseq s k') = CC.Kseq s0 k0' ->
-        exists mm', ev_star ge (CC.State f s k' ve te mm) m nil (CC.State f s0 k0' ve te mm') m.
-Proof.
- intros.
- destruct (dec_skip s). subst. simpl in *.
- revert mm; induction k'; try solve [inv H].
- destruct (dec_skip s).
- { subst. simpl in *.
-   replace nil with (@nil mem_event ++ nil) by reflexivity.
-   destruct (IHk' H m) as [mm' ?]; exists mm'.
-   econstructor 2; eauto. constructor. }
- { rewrite strip_skip'_not in * by auto.
-   inv H. replace nil with (@nil mem_event ++ nil) by reflexivity.
-   intro; exists m.
-   econstructor 2; eauto. constructor. constructor 1. }
- { rewrite strip_skip'_not in H by auto. inv H. exists mm; constructor 1. }
-Qed.
-
-Lemma evstep_continue_strip:
-  forall ge f k ve te m,
-           ev_star ge (CC.State f Scontinue k ve te m) m nil
-               (CC.State f Scontinue (strip_skip' k) ve te m) m.
-Proof.
-intros.
-induction k; simpl; try (constructor 1).
-destruct (dec_skip s).
-{ subst. replace nil with (@nil mem_event ++ nil) by reflexivity.
-  eapply ev_star_trans.
-  apply ev_star_one. simpl. apply clc_evstep_continue_seq.
-  auto. }
-destruct s; try congruence; constructor 1.
-Qed.
-
-Lemma break_evstrip:
- forall ge f ve te m k mm,
-     exists mm', ev_star ge (CC.State f Sbreak k ve te mm) m nil (CC.State f Sbreak (strip_skip' k) ve te mm') m.
-Proof.
-  induction k; try solve [eexists; constructor 1]. intros.
-  destruct (dec_skip s).
-  { subst. replace nil with (@nil mem_event ++ nil) by reflexivity.
-    destruct (IHk m) as [mm' ?]; exists mm'.
-    econstructor 2. constructor. eauto. } 
-  { rewrite strip_skip'_not; auto. exists mm; constructor 1. }
-Qed.
-
-Lemma Clight_new_ev_sim : forall ge c1 m ev c1' m',
-    event_semantics.ev_step (@semSem (Clight_newSem ge)) c1 m ev c1' m' ->
-    forall c2, match_states c1 (fst (CC'.CC_state_to_CC_core c2)) ->
-    exists c2', ev_plus ge c2 m ev c2' m' /\
-      match_states c1' (fst (CC'.CC_state_to_CC_core c2')).
-  Proof.
-    (* based on Clight_sim.Clightnew_Clight_sim_eq_noOrder_SSplusConclusion *)
-intros. simpl in H. revert c2 H0. induction H; intros.
-
-{ (* step_assign *)
-  destruct c2; simpl in *; inv H4. rename k0 into k'.
-  simpl strip_skip in H6.
-  destruct (exec_skipsT ge H6 f e le m m0) as [k2 [m2 [K2 STAR]]]; simpl; auto.
-  exists (CC_core_to_CC_state (CC'.CC_core_State f Sskip k2 e le) m').
-  rewrite CC'.CC_core_CC_state_1; simpl. split.
-  + replace (T1++T2++T3) with (nil ++ (T1++T2++T3)) by reflexivity.
-    eapply ev_star_plus_trans; try eassumption;
-      apply ev_plus_one; econstructor; eauto.
-  + constructor. apply CUR. rewrite  K2 in H6. inv H6. assumption. }
-
-{ (* step_set *)
-  destruct c2; simpl in *; inv H0. rename k0 into k'. 
-  destruct (exec_skipsT ge H2 f e le m m0) as [k2 [m2 [K2 STAR]]]; simpl; auto.
-  exists (CC_core_to_CC_state (CC'.CC_core_State f Sskip k2 e (PTree.set id v le)) m).
-  rewrite CC'.CC_core_CC_state_1; simpl. split. 
-  + replace T with (nil ++ T) by reflexivity.
-    eapply ev_star_plus_trans; try eassumption;
-      apply ev_plus_one; econstructor; eauto.
-  + rewrite K2 in H2; inv H2; constructor; auto. }
-
-{ (* step_call_internal *)
-  destruct c2; simpl in *; inv H7. rename k0 into k'. 
-  destruct (exec_skipsT ge H9 f0 e le m m0) as [k2 [m2 [K2 STAR]]]; simpl; auto.
-  rewrite K2 in H9; inv H9. simpl in CUR.
-  exists (CC_core_to_CC_state (CC'.CC_core_State f (fn_body f) (CC.Kcall optid f0 e le k2) ve' le') m1).
-  rewrite CC'.CC_core_CC_state_1; simpl. split. 
-  + replace (T1++T2++T3) with (nil ++ (T1++T2++T3)) by reflexivity.
-    eapply ev_star_plus_trans; try eassumption.
-    replace (T1++T2++T3) with ((T1++T2)++T3) by (rewrite app_assoc; trivial).
-    eapply ev_plus_two. simpl. econstructor; try eassumption.
-    econstructor; eauto.
-    apply list_norepet_app in H4. destruct H4 as [? [? ?]].
-    econstructor; auto.
-  + constructor.
-    simpl; auto.
-    apply match_cont_strip. simpl. constructor; auto. }
-
-{ (* step_call_external *)
-  destruct c2; simpl in *; inv H3. rename k0 into k'. 
-  destruct (exec_skipsT ge H5 f e le m m0) as [k2 [m2 [K2 STAR]]]; simpl; auto.
-  rewrite K2 in H5; inv H5. simpl in CUR.
-  exists (CC_core_to_CC_state (CC'.CC_core_Callstate
-                                 (External ef tyargs tyres cc) vargs (CC.Kcall optid f e le k2)) m).
-  rewrite CC'.CC_core_CC_state_1; simpl. split. 
-  + replace (T1++T2) with (nil ++ (T1++T2)) by reflexivity.
-    eapply ev_star_plus_trans; try eassumption;
-      apply ev_plus_one; econstructor; eauto.
-  + econstructor; eauto. }
-
-{ (* step_seq *)
-  destruct c2; simpl in *; inv H0. rename k0 into k'. 
-  destruct (exec_skipsT ge H2 f e le m m0) as [k2 [m2 [K2 STAR]]]; simpl; auto.
-  rewrite K2 in H2; inv H2. 
-  destruct (IHcl_evstep (CC_core_to_CC_state (CC'.CC_core_State f s1 (CC.Kseq s2 k2) e le) m))
-    as [st2 [? ?]]; clear  IHcl_evstep.
-  + repeat constructor; auto.
-    apply match_cont_strip.  apply match_cont_strip.  auto.
-  + exists st2; split; auto.
-    replace T with (nil ++ (nil++T)) by reflexivity.
-    eapply ev_star_plus_trans; try eassumption.
-      eapply ev_plus_trans. apply ev_plus_one. constructor. eassumption. }
-
-{ (* step_skip *)
-  destruct c2; simpl in *; inv H0. rename k0 into k'. 
-  simpl strip_skip in H2.
-  remember (strip_skip k) as k0.
-  destruct k0.
-  elimtype False; clear - H Heqk0.
-  revert H; induction k; intros. inv H.
-  forget (a::k) as k';  clear - Heqk0 H.
-  remember (State e le k') as s.
-  revert e le k' Heqs Heqk0; induction H; intros; inv Heqs; simpl in *; try congruence.
-  eapply IHcl_evstep. reflexivity. auto.
-  remember (strip_skip' (CC.Kseq s k')) as k0'.
-  destruct k0'; inv H2;
-    try solve [rewrite <- strip_evstep in H; rewrite <- Heqk0 in H; inv H].
-  +
-    assert (s0<>Sskip).
-    clear- Heqk0; intro; subst.
-    revert Heqk0; induction k; simpl; intros. inv Heqk0. destruct a; try solve [inv Heqk0]; auto. destruct s; inv Heqk0; auto.
-    destruct (IHcl_evstep (CC_core_to_CC_state (CC'.CC_core_State f s k' e le) m0))
-      as [st2 [? ?]]; clear  IHcl_evstep.
-    constructor; auto. rewrite <- Heqk0. rewrite <- Heqk0'.
-    constructor 2; auto. simpl in H2.
-    exists st2; split; auto.
-  +
-    destruct s; inv Heqk0'.
-    edestruct (ev_strip_skip'_loop1) as [m2 STAR]; eauto.
-    destruct (IHcl_evstep (CC_core_to_CC_state (CC'.CC_core_State f Sskip (CC.Kloop1 s0 s1 k0') e le) m2))
-      as [st2 [? ?]]; clear  IHcl_evstep.
-    constructor; auto. simpl. rewrite <- Heqk0. constructor. auto.
-    exists st2; split; auto.
-    simpl in H0. inv H0. rename ev1 into T1; rename ev2 into T2.
-    eapply ev_plus_star_trans; try apply H5.
-    clear - STAR H4.
-    replace T1 with (nil++T1) by reflexivity.
-    eapply ev_star_plus_trans; [ | apply ev_plus_one; eauto ].
-    apply STAR.
-  +
-    destruct s; inv Heqk0'.
-    edestruct evstrip_skip'_loop2 as [m2 STAR]; eauto.
-    destruct (IHcl_evstep (CC_core_to_CC_state (CC'.CC_core_State f Sskip (CC.Kloop2 s0 s1 k0') e le) m2))
-      as [st2 [? ?]]; clear IHcl_evstep.
-    econstructor; eauto. rewrite <- Heqk0. constructor. auto.
-    exists st2; split; auto.
-    replace T with (nil++T) by reflexivity.
-    eapply ev_star_plus_trans; try apply H0.
-    apply STAR.
-  +
-    destruct s; inv Heqk0'.
-    destruct (IHcl_evstep (CC_core_to_CC_state (CC'.CC_core_State f Sskip (CC.Kcall o f0 e0 t k0') e le) m0))
-      as [st2 [? ?]]; clear IHcl_evstep.
-    constructor; auto. rewrite <- Heqk0. constructor; auto.
-    exists st2; split; auto.
-    inv H0.
-    eapply ev_plus_star_trans; [ | apply H5].
-    inv H4.
-    replace ([Free (blocks_of_env ge e)]) with (nil ++ [Free (blocks_of_env ge e)]) by reflexivity.
-    edestruct evstrip_skip'_call as [m2' STAR]; eauto.
-    eapply ev_star_plus_trans; [apply STAR | ].
-    apply ev_plus_one. constructor; auto. }
-    
-{ (* step_continue *)
-  destruct c2; simpl in *; inv H0. rename k0 into k'. 
-  simpl strip_skip in H2; inv H2.
-  +
-    change (CC.Kseq Scontinue k'0 = strip_skip' (CC.Kseq s k')) in H4.
-    symmetry in H4.
-    rewrite continue_cont_skip in *.
-    simpl in CUR.
-    rewrite <- current_function_strip in CUR.
-    forget (strip_skip k) as k0. clear k. rename k0 into k.
-    generalize (continue_cont_is k); case_eq (continue_cont k); intros; try contradiction.
-    rewrite H0 in H; inv H.
-    destruct c; try contradiction. destruct l; try contradiction. destruct c; try contradiction.
-    subst s0.
-    assert (exists m2, ev_star ge (CC.State f s k' e le m0) m nil
-                 (CC.State f Scontinue k'0 e le m2) m) as [m2 X1].
-    { clear - H4.
-      destruct (dec_skip s). subst. simpl in H4.
-      edestruct evexec_skips' with (s := Sskip) as [m2 STAR]; eauto.
-      rewrite strip_skip'_not in H4 by auto. inv H4. eexists; constructor. }
-    assert (exists m3, ev_star ge (CC.State f Scontinue k'0 e le m2) m nil
-                 (CC.State f Scontinue (strip_skip' k'0) e le m3) m) as [m3 X2].
-    { clear.
-      revert m2; induction k'0; try solve [eexists; constructor 1].
-      destruct (dec_skip s).
-      { subst. simpl in *.
-        destruct (IHk'0 m).
-        replace nil with (@nil mem_event ++ nil) by reflexivity. eexists; econstructor 2.
-        constructor. apply H. }
-      rewrite strip_skip'_not; auto. eexists; constructor 1. }
-    generalize (ev_star_trans ge X1 X2); clear X1 X2; intro.
-    clear H4.
-    forget (strip_skip' k'0) as k0'; clear k'0.
-    assert (precontinue_cont k = Kloop1 s1 s2 :: l).
-    revert H0; clear; induction k; simpl; try congruence.  destruct a; try congruence; auto.
-    assert (K1': exists k1' m4,
-               ev_star ge (CC.State f Scontinue k0' e le m3) m nil
-                    (CC.State f Scontinue k1' e le m4) m /\
-               match_cont (Kseq Scontinue :: Kloop1 s1 s2 :: l) k1'). {
-      clear - H1 H0.
-      revert m3 H0; induction H1; simpl; intros; try congruence.
-      { destruct (IHmatch_cont m) as [k1' [? [? ?]]].
-        rewrite <- continue_cont_skip; auto.
-        do 2 eexists. split; [ | eassumption].
-        replace nil with (@nil mem_event ++ nil) by reflexivity.
-        eapply ev_star_trans; try apply H.
-        clear.
-        replace nil with (@nil mem_event ++ nil) by reflexivity.
-        eapply ev_star_trans. apply ev_star_one.
-        simpl. apply clc_evstep_continue_seq.
-        apply evstep_continue_strip. }
-      { inv H0.
-        do 2 econstructor; split. constructor 1.  constructor.  auto. }
-      { edestruct IHmatch_cont as [k1' [? [? ?]]].
-        rewrite <- continue_cont_skip; auto.
-        do 2 econstructor. split; [ | eassumption].
-        replace nil with (@nil mem_event ++ nil) by reflexivity.
-        eapply ev_star_trans; try apply H.
-        replace nil with (@nil mem_event ++ nil) by reflexivity.
-        eapply ev_star_trans.
-        + apply ev_star_one. simpl.
-         apply clc_evstep_continue_switch.
-        + apply evstep_continue_strip. }
-    }
-    destruct K1' as [k1' [? [STAR1 K1]]].
-    generalize (ev_star_trans ge H2 STAR1); clear H2 STAR1; intro STAR.
-    rewrite H0 in *.
-    assert (CUR': match current_function l with
-                  | Some f' => f' = f
-                  | None => True
-                  end). {
-      clear - CUR H0. revert CUR H0; induction k; simpl; intros.
-      inv H0.
-      destruct a; try discriminate; auto.
-      apply IHk. auto. auto. inv H0. auto.
-      apply IHk; auto.
-    }
-    clear H1 CUR k H0 H3.
-    inv K1. inv H3. simpl in *.
-    destruct (IHcl_evstep (CC_core_to_CC_state (CC'.CC_core_State f s2 (CC.Kloop2 s1 s2 k'0) e le) m))
-                      as [st2 [? ?]]; clear IHcl_evstep.
-    constructor; auto. apply match_cont_strip. constructor. auto.
-    exists st2; split; auto.
-    replace T with (nil++T) by reflexivity.
-    eapply ev_star_plus_trans; [apply STAR | ].
-    replace T with (nil++T) by reflexivity.
-    eapply ev_star_plus_trans; [ | apply H0].
-    replace nil with (@nil mem_event ++ nil) by reflexivity.
-    apply ev_star_one. constructor. auto.
- +
-   change (CC.Kloop1 s0 e3 k'0 = strip_skip' (CC.Kseq s k')) in H1.
-   destruct (dec_skip s); [ | destruct s; try congruence; inv H1].
-   subst s.
-   simpl in H.
-   simpl in H1.
-   simpl in *.
-   assert (exists m2, ev_star ge (CC.State f Sskip k' e le m0) m nil
-                (CC.State f Sskip (CC.Kloop1 s0 e3 k'0) e le m2) m) as [m2 STAR].
-   { rewrite H1; clear.
-     revert m0; induction k'; intros; try solve [eexists; constructor 1].
-     destruct (dec_skip s).
-     { subst. simpl in *.
-       replace nil with (@nil mem_event ++ nil) by reflexivity.
-       destruct (IHk' m). eexists; econstructor 2; eauto.
-       constructor. }
-     { rewrite strip_skip'_not; auto. eexists; constructor 1. } }
-   forget (CC.State f Sskip k' e le m0) as st1.
-   clear k' H1.
-   assert (PLUS: ev_plus ge st1 m nil (CC.State f e3 (CC.Kloop2 s0 e3 k'0) e le m) m).
-   {
-     replace nil with (@nil mem_event ++ nil) by reflexivity.
-     eapply ev_star_plus_trans; try apply STAR.
-     replace nil with (@nil mem_event ++ nil) by reflexivity.
-     econstructor. econstructor. auto. constructor 1. }
-   clear STAR.
-   destruct (IHcl_evstep (CC_core_to_CC_state(CC'.CC_core_State f e3 (CC.Kloop2  s0 e3 k'0) e le) m))
-     as [st2 [? ?]]; clear  IHcl_evstep.
-   { constructor; auto. apply match_cont_strip; constructor; auto. }
-   { exists st2; split; auto.
-     replace T with (nil ++ T) by reflexivity. simpl in H0.
-     eapply ev_plus_trans; eauto. } }
-
-{ (* step_break *)
-  destruct c2; simpl in *; inv H0. rename k0 into k'. 
-  simpl strip_skip in H2; inv H2.
-  change (CC.Kseq Sbreak k'0 = strip_skip' (CC.Kseq s k')) in H4.
-  symmetry in H4.
-  rewrite <- break_cont_skip in *.
-  simpl in CUR.
-  rewrite <- current_function_strip in CUR.
-  forget (strip_skip k) as k0. clear k. rename k0 into k.
-  simpl.
-  destruct (evexec_skips' ge f s k' Sbreak k'0 e le m m0 H4) as [m1 ?].
-  forget (CC.State f s k' e le m0) as st1.
-  clear k' H4.
-  edestruct (break_evstrip ge f e le m k'0 m1) as [m2 ?].
-  pose proof (ev_star_trans ge H0 H2); clear H0 H2.
-  forget (strip_skip' k'0) as k0'; clear k'0.
-  assert (X:exists k1',
-             ev_plus ge (CC.State f Sbreak k0' e le m2) m nil
-                  (CC.State f Sskip k1' e le m) m
-             /\ match_cont (strip_skip (break_cont k)) (strip_skip' k1')). {
-    clear - H H1. rename H1 into H2.
-    revert m2 H; induction H2; intros; try solve [inv H].
-    { rewrite break_cont_skip in *. simpl in H.
-      edestruct break_evstrip as [m1 ?].
-      destruct (IHmatch_cont m1 H) as [k1' [? ?]]; clear IHmatch_cont. simpl.
-      exists k1'; split; auto.
-      replace nil with (@nil mem_event ++ nil) by reflexivity.
-      eapply ev_star_plus_trans, H1.
-      replace nil with (@nil mem_event ++ nil) by reflexivity.
-      econstructor 2; eauto. constructor. }
-      
-    { simpl  in *.
-      replace nil with (@nil mem_event ++ nil) by reflexivity.
-      exists k'; split. econstructor.
-      simpl. eapply clc_evstep_break_loop1. constructor 1. auto. }
-
-
-    { simpl in *. 
-      replace nil with (@nil mem_event ++ nil) by reflexivity.
-      exists k'; split. econstructor. simpl. eapply clc_evstep_break_loop2. auto.
-      constructor 1; auto.
-      auto. }
-
-    { simpl in *. 
-      replace nil with (@nil mem_event ++ nil) by reflexivity.
-      exists k'; split. econstructor. simpl. eapply clc_evstep_skip_break_switch. auto.
-      constructor 1; auto.
-      auto. }
-  }
-  
-  destruct X as [k1' [? ?]].
-  destruct (IHcl_evstep (CC_core_to_CC_state (CC'.CC_core_State f Sskip k1' e le) m))
-    as [st2 [? ?]]; clear IHcl_evstep.
-  { constructor; auto.
-    clear - H CUR.
-    revert CUR; induction  k; intros. apply I.
-    destruct a; simpl in *; auto. apply IHk; auto. }
-  { exists st2; split; auto.
-    simpl in H4.
-    replace T with (nil ++ T) by reflexivity. 
-    eapply ev_star_plus_trans; [ | eassumption].
-    replace nil with (@nil mem_event ++ nil) by reflexivity.
-    eapply ev_star_trans; [eassumption | ]. 
-    replace nil with (@nil mem_event ++ nil) by reflexivity.
-    apply ev_plus_star; eassumption. } }
-
-{ (* step_ifthenelse *)
-  destruct c2; simpl in *; inv H1. rename k0 into k'. 
-  simpl strip_skip in H3; inv H3.
-  change (CC.Kseq (Sifthenelse a s1 s2) k'0 = strip_skip' (CC.Kseq s k')) in H5.
-  assert (exists m2, ev_star ge (CC.State f s k' e le m0) m nil (CC.State f (Sifthenelse a s1 s2) k'0 e le m2) m)
-    as [m2 STAR]. {
-     clear - H5.
-     revert m0 H5; induction k'; intros; try solve [ destruct s; inv H5; eexists; constructor 1].
-     destruct (dec_skip s).
-     { subst s.
-       destruct (dec_skip s0).
-       { subst s0. simpl in *.
-         replace nil with (@nil mem_event ++ nil) by reflexivity.
-         destruct (IHk' m); auto.
-         eexists; eapply ev_star_trans; eauto.
-         replace nil with (@nil mem_event ++ nil) by reflexivity. apply ev_star_one.
-         constructor. }
-       { change (strip_skip' (CC.Kseq Sskip (CC.Kseq s0 k'))) with
-               (strip_skip' (CC.Kseq s0 k')) in H5.
-         rewrite strip_skip'_not in H5 by auto.
-         inv H5.
-         replace nil with (@nil mem_event ++ nil) by reflexivity. eexists; apply ev_star_one.
-         constructor. } }
-     { rewrite strip_skip'_not in * by auto.
-       inv H5. eexists; constructor 1. }
-  }
-  exists (CC_core_to_CC_state (CC'.CC_core_State f (if b then s1 else s2) k'0 e le) m); split; auto.
-  { 
-    replace T with (nil ++ T) by reflexivity. eapply ev_star_plus_trans; try apply STAR.
-    replace nil with (@nil mem_event ++ nil) by reflexivity. 
-    apply ev_plus_one. econstructor; eauto. }
-  { constructor; auto.
-    apply match_cont_strip; auto. } }
-
-{ (* step_loop *)
-  destruct c2; simpl in *; inv H0. rename k0 into k'.
-  inv H1. inv H3.
-  change (CC.Kseq (Sloop s1 s2) k'0 = strip_skip' (CC.Kseq s k')) in H1.
-  destruct (evexec_skips' ge f _ _ _ _ e le m m0 (@eq_sym _ _ _ H1)).
-  exists (CC_core_to_CC_state (CC'.CC_core_State f s1 (CC.Kloop1 s1 s2 k'0) e le) m); split.
-  { replace nil with (@nil mem_event ++ nil) by reflexivity.
-    eapply ev_star_plus_trans; try apply H.
-    replace nil with (@nil mem_event ++ nil) by reflexivity.
-    apply ev_plus_one. simpl. eapply clc_evstep_loop; eauto. }
-  { constructor; auto. apply match_cont_strip; constructor; auto. } }
-
-{ (* step_loop2 *)
-  destruct c2; simpl in *; inv H0. rename k0 into k'.
-  inv H1.
-  destruct s0; inv H4.
-  destruct (evstrip_skip'_loop2 ge f e le m _ _ _ _ m0 H1).
-  exists (CC_core_to_CC_state (CC'.CC_core_State f s (CC.Kloop1 s a3 k'0) e le) m); split.
-  + replace nil with (@nil mem_event ++ nil) by reflexivity.
-    eapply ev_star_plus_trans; try apply H.
-    replace nil with (@nil mem_event ++ nil) by reflexivity.
-    econstructor. simpl. eapply clc_evstep_skip_loop2; eauto.
-    replace nil with (@nil mem_event ++ nil) by reflexivity.
-    apply ev_star_one. simpl. eapply clc_evstep_loop; eauto.
-  + constructor; auto. apply match_cont_strip. constructor. auto. }
-
-{ (* step_return *)
-  destruct c2; simpl in *; inv H3. rename k0 into k'0.
-  remember (strip_skip' (CC.Kseq s k'0)) as k3. simpl in CUR, H5.
-  inv H5.
-  { (*first case*)
-    destruct (evexec_skips' ge f0 _ _ _ _ e le m m0 (@eq_sym _ _ _ H4)) as [? H99].
-    assert (f0=f).
-    { simpl in CUR; clear - CUR H.
-      revert H CUR; induction k; intros. inv H. simpl in *. destruct a; auto. inv CUR; auto. inv H; auto.
-    }
-    subst f.
-    generalize (match_cont_call_strip k k'1); intro.
-    spec H3; [congruence |]. spec H3; [auto |].
-    generalize H3; rewrite H; intro.
-    inv H5.
-    +  elimtype False; clear - H10.
-       revert H10; induction k'1; simpl; intros; congruence.
-    + destruct optexp;  [destruct H1 as [v [? ?]] | ]; (destruct optid; destruct H2 as [H2 H2'];
-               try solve [contradiction H2; auto]; subst te'' ).
-    -   eexists (CC_core_to_CC_state (CC'.CC_core_State f Sskip k'2 ve' (PTree.set i v' te')) m').
-        split.
-        { replace (T ++ [Free (blocks_of_env ge e)]) with ((T ++ [Free (blocks_of_env ge e)]) ++ nil) by (rewrite app_nil_r; trivial).
-          apply (ev_star_plus_trans ge H99). (*with (s2:=CC.State f0 (Sreturn (Some e)) k'1 ve te m).  apply H99. *)
-          eapply (@ev_plus_trans ge) with (s2:=CC.Returnstate v' (CC.call_cont k'1) m').
-          eapply ev_plus_one. simpl. eapply clc_evstep_return_1; eauto. 
-          eapply ev_plus_one. simpl. rewrite <- H13.
-          eapply clc_evstep_returnstate. }
-        constructor; auto.
-    -   eexists (CC_core_to_CC_state (CC'.CC_core_State f Sskip k'2 ve' te') m').
-        split.
-        { replace (T ++ [Free (blocks_of_env ge e)]) with ((T ++ [Free (blocks_of_env ge e)]) ++ nil) by (rewrite app_nil_r; trivial).
-          eapply (ev_star_plus_trans ge H99). (* with (s2:=CC.State f0 (Sreturn (Some e)) k'1 ve te m). apply H99. *)
-          eapply (@ev_plus_trans ge) with (s2:=CC.Returnstate v' (CC.call_cont k'1) m').
-          eapply ev_plus_one. simpl. econstructor; eauto.
-          eapply ev_plus_one. simpl. rewrite <- H13. eapply clc_evstep_returnstate. }
-        constructor; auto.
-    -   destruct H1; subst.
-        eexists (CC_core_to_CC_state (CC'.CC_core_State f Sskip k'2 ve' (CC.set_opttemp (Some i) Vundef te')) m').
-        split.
-        { eapply (ev_star_plus_trans ge H99).  (*with (s2:=CC.State f0 (Sreturn None) k'1 ve te m).  apply H99. *)
-          replace [Free (blocks_of_env ge e)] with (([Free (blocks_of_env ge e)] ++ nil) ++ nil)
-            by (rewrite app_nil_r; trivial).  
-          eapply (@ev_plus_trans ge) with (s2:=CC.Returnstate Vundef (CC.call_cont k'1) m').
-          eapply ev_plus_one. simpl. econstructor; eauto.
-          eapply ev_plus_one. simpl. rewrite <- H13.
-          apply clc_evstep_returnstate. } 
-        simpl. constructor 1. auto. simpl.  auto.
-    - destruct H1; subst.
-      eexists (CC_core_to_CC_state (CC'.CC_core_State f Sskip k'2 ve' te') m').
-      split.
-      { eapply (ev_star_plus_trans ge H99).
-        replace [Free (blocks_of_env ge e)] with (([Free (blocks_of_env ge e)] ++ nil) ++ nil)
-          by (rewrite app_nil_r; trivial). 
-        eapply (@ev_plus_trans) with (s2:=CC.Returnstate Vundef (CC.call_cont k'1) m').
-        eapply ev_plus_one. simpl. econstructor; eauto.
-        eapply ev_plus_one. simpl. rewrite <- H13.
-        apply clc_evstep_returnstate. }
-      simpl. constructor 1. auto. simpl.  auto. }
-  { (*second case*)
-    destruct H1; subst. destruct optid; destruct H2 as [_ H2]; subst te''.
-    { simpl in H. inv H. simpl in CUR. symmetry in CUR; inv CUR. 
-      destruct s; inv H4.
-      assert (exists m2, ev_star ge (CC.State f Sskip k'0 e le m0) m nil
-                            (CC.State f Sskip (CC.Kcall (Some i) f1 ve' te' k'1) e le m2) m) as [m2 STAR].
-      { clear - H1.
-        revert m0 H1; induction k'0; intros; try solve [inv H1].
-        destruct (dec_skip s). subst s. simpl in H1.
-        replace nil with (@nil mem_event ++ nil) by reflexivity.
-        destruct (IHk'0 m); auto.
-        eexists; eapply ev_star_trans; eauto.
-        replace nil with (@nil mem_event ++ nil) by reflexivity.
-        apply ev_star_one. simpl. constructor; auto.
-        rewrite strip_skip'_not in H1 by auto. rewrite <- H1. eexists; constructor 1.
-        simpl in H1. inv H1. eexists; constructor 1. }
-      eexists; split.
-      { eapply ev_star_plus_trans. apply STAR.
-        replace [Free (blocks_of_env ge e)] with ([Free (blocks_of_env ge e)] ++ nil)
-          by (rewrite app_nil_r; trivial).
-        eapply ev_plus_two.
-        + simpl. eapply clc_evstep_skip_call; simpl; eauto.
-        + simpl. apply clc_evstep_returnstate. }
-      econstructor; eauto. }
-    { simpl in H. inv H. simpl in CUR. symmetry in CUR; inv CUR.
-      destruct s; inv H4.
-      assert (exists m2, ev_star ge (CC.State f Sskip k'0 e le m0) m nil
-                            (CC.State f Sskip (CC.Kcall None f1 ve' te' k'1) e le m2) m) as [m2 STAR].
-      { clear - H1.
-        revert m0 H1; induction k'0; intros; try solve [inv H1].
-        destruct (dec_skip s). subst s. simpl in H1.
-        replace nil with (@nil mem_event ++ nil) by reflexivity.
-        destruct (IHk'0 m); auto.
-        eexists; eapply ev_star_trans; eauto.
-        replace nil with (@nil mem_event ++ nil) by reflexivity.
-        apply ev_star_one. simpl. constructor; auto.
-        rewrite strip_skip'_not in H1 by auto. rewrite <- H1. eexists; constructor 1.
-        simpl in H1. inv H1. eexists; constructor 1. }
-      eexists; split.
-      { eapply ev_star_plus_trans. apply STAR.
-        replace [Free (blocks_of_env ge e)] with ([Free (blocks_of_env ge e)] ++ nil)
-          by (rewrite app_nil_r; trivial).
-        eapply ev_plus_two.
-        + simpl. eapply clc_evstep_skip_call; simpl; eauto.
-        + simpl.  apply clc_evstep_returnstate. }
-      econstructor; eauto. } } }
-
-{ (* step_switch *)
-  destruct c2; simpl in *; inv H1. rename k0 into k'.
-  simpl strip_skip in H3.
-  remember (CC.Kseq s k') as k0'.
-  inv H3.
-  exists  (CC'.CC_core_to_CC_state (CC'.CC_core_State f (seq_of_labeled_statement (select_switch n sl)) 
-              (Clight.Kswitch k'0) e le) m); split.
-  { destruct (evexec_skips' ge f _ _ _ _ e le m m0 (@eq_sym _ _ _ H5)) as [? H99].
-    replace T with (nil++T) by reflexivity. eapply ev_star_plus_trans; try apply H99.
-    eapply ev_plus_one. simpl. econstructor; eassumption. }
-  { simpl. constructor; auto. apply match_cont_strip. constructor; auto. } }
-  
-{ (* step_label *)
-  destruct c2; simpl in *; inv H0. rename k0 into k'. 
-  remember (CC.Kseq s0 k') as k0'. inv H2.
-  destruct (IHcl_evstep (CC_core_to_CC_state (CC'.CC_core_State f s k'0 e le) m)) as [st2 [? ?]]; clear IHcl_evstep.
-  { constructor; auto. apply match_cont_strip. auto. }
-  exists st2; split; auto. simpl in H0.
-  replace T with (nil++T) by reflexivity.
-  eapply ev_star_plus_trans; try eassumption.
-  replace nil with (@nil mem_event ++ nil) by reflexivity.
-  destruct (evexec_skips' ge f _ _ _ _ e le m m0 (@eq_sym _ _ _ H4)).
-  eapply ev_star_trans; eauto.
-  apply ev_star_one. constructor. } 
-
-{ (* step_goto *)
-  destruct c2; simpl in *; inv H0. 
-  remember (CC.Kseq s k0) as k0'. inv H2.
-  generalize (match_cont_call_strip k k'0(*k'1*)); intro.
-  spec H0.
-  { clear - CUR. apply (call_cont_nonnil _ _ CUR). }
-  specialize (H0 H1).
-  rewrite <- strip_call' in H0.
-  change (Kseq (Sreturn None) :: call_cont k) with (strip_skip (Kseq (Sreturn None) :: call_cont k)) in H0.
-  destruct (match_find_label _ _ _ _ _ H0 H) as [s2 [k2' [? ?]]].
-  exists (CC'.CC_core_to_CC_state (CC'.CC_core_State f s2 k2' e le) m); split.
-  { simpl in CUR0. inversion2 CUR CUR0.
-    destruct (evexec_skips' ge f _ _ _ _ e le m m0 (@eq_sym _ _ _ H4)) as [? H99].
-    replace nil with (@nil mem_event ++ nil) by reflexivity.
-    eapply ev_star_plus_trans; try apply H99.
-    apply ev_plus_one. constructor; auto. }
-  constructor; auto.
-  clear - CUR H. forget (fn_body f) as s.
-  rewrite <- current_function_call_cont in CUR.
-  change (current_function (Kseq (Sreturn None) :: call_cont k) = Some f) in CUR.
-  forget (Kseq (Sreturn None) :: call_cont k) as k0. clear - CUR H.
-  rewrite (current_function_find_label _ _ _ _ _ CUR H). auto.
-  apply match_cont_strip1. auto. }
-Qed.
 
