floyd/forward_lemmas.v
@@ -24,6 +24,7 @@ Lemma semax_func_cons_ext_vacuous:
          (argsig : typelist) (retsig : type)
          (G' : funspecs) cc b,
        (id_in_list id (map fst fs)) = false ->
+       ef_inline ef = false ->
        ef_sig ef =
        {|
          sig_args := typlist_of_typelist (type_of_params (arglist 1 argsig));
