Makefile
@@ -567,12 +567,12 @@ floyd/floyd.coq: floyd/proofauto.vo
 	coqtop $(COQFLAGS) -load-vernac-object floyd/proofauto -outputstate floyd/floyd -batch
 
 .depend depend:
-	@echo "Copying Clight_core.v ... "
-ifeq ($(COMPCERT), compcert_new)
-	@cp -p concurrency/shim/Clight_core.v veric/Clight_core.v
-else
-	@cp -p veric/Clight_core_standard.v veric/Clight_core.v
-endif
+#	@echo "Copying Clight_core.v ... "
+# ifeq ($(COMPCERT), compcert_new)
+#	@cp -p concurrency/shim/Clight_core.v veric/Clight_core.v
+# else
+# 	@cp -p veric/Clight_core_standard.v veric/Clight_core.v
+# endif
 	@echo 'coqdep ... >.depend'
 	$(COQDEP) $(COMPCERT_R_FLAGS) 2>&1 >.depend `find $(addprefix $(COMPCERT)/,$(COMPCERTDIRS))  -name "*.v"` | grep -v 'Warning:.*found in the loadpath' || true
 ifeq ($(COMPCERT), compcert_new)
